

Cosets and Lagrange's Theorem

Our current goal is to generalize the Fundamental Theorem for Cyclic Groups, which said that a cyclic group of order $|G| = n$ has a single subgroup of order $|H| = d$ for each divisor d of n . This statement has three parts.

1. Order of subgroups divides order of cyclic groups.
2. There **exists** a subgroup with $|H| = d$ for each divisor d of $|G|$.
(In particular, there is an **element** of order d for each divisor.)
3. There is **only one** such H .

Generalizing the first of these to all groups is done by **Lagrange's Theorem**, proven using **cosets**.

Definition. For each $g \in G$, a subgroup $H < G$ has

$$\text{left coset } gH = \{gh \mid h \in H\} \quad \text{and} \quad \text{right coset } Hg = \{hg \mid h \in H\}$$

We'll usually focus on **left** cosets. If we say just "coset" then we mean "**left** coset".

Remark. Sometimes in set theory people say "co-set" to mean "complementary set" (i.e. everything other than the set). **This is different!** Our "coset" is more like a "parallel set".

Example. In \mathbb{Z}_6 consider the subgroup $\langle 3 \rangle = \{0, 3\}$. This has the following (three) cosets.

- $0 + \langle 3 \rangle = \{0, 3\}$
- $1 + \langle 3 \rangle = \{1, 4\}$
- $2 + \langle 3 \rangle = \{2, 5\}$
- $3 + \langle 3 \rangle = \{3, 0\} = 0 + \langle 3 \rangle$
- $4 + \langle 3 \rangle = \{4, 1\} = 1 + \langle 3 \rangle$
- $5 + \langle 3 \rangle = \{5, 2\} = 2 + \langle 3 \rangle$

Example. In \mathbb{Z}_6 consider the subgroup $\langle 2 \rangle = \{0, 2, 4\}$. This has the following (two) cosets.

- $0 + \langle 2 \rangle = \{0, 2, 4\}$
- $1 + \langle 2 \rangle = \{1, 3, 5\}$
- $2 + \langle 2 \rangle = \{2, 4, 0\} = 0 + \langle 2 \rangle$
- $3 + \langle 2 \rangle = \{3, 5, 1\} = 1 + \langle 2 \rangle$
- $4 + \langle 2 \rangle = \{4, 0, 2\} = 0 + \langle 2 \rangle$
- $5 + \langle 2 \rangle = \{5, 3, 1\} = 1 + \langle 2 \rangle$

Example. In S_3 consider the subgroup $\langle (1\ 2) \rangle = \{(1), (1\ 2)\}$. This has the following (three) cosets.

- $(1) \langle (1\ 2) \rangle = \{(1), (1\ 2)\}$
- $(1\ 2) \langle (1\ 2) \rangle = \{(1\ 2), (1)\}$
- $(1\ 3) \langle (1\ 2) \rangle = \{(1\ 3), (1\ 2\ 3)\}$
- $(1\ 2\ 3) \langle (1\ 2) \rangle = \{(1\ 2\ 3), (1\ 3)\}$
- $(2\ 3) \langle (1\ 2) \rangle = \{(2\ 3), (1\ 3\ 2)\}$
- $(1\ 3\ 2) \langle (1\ 2) \rangle = \{(1\ 3\ 2), (2\ 3)\}$

Example. In S_3 consider the subgroup $\langle (1\ 2\ 3) \rangle = \{(1), (1\ 2\ 3), (1\ 3\ 2)\}$. This has the following two cosets.

- $(1) \langle (1\ 2\ 3) \rangle = \{(1), (1\ 2\ 3), (1\ 3\ 2)\} = (1\ 2\ 3) \langle (1\ 2\ 3) \rangle = (1\ 3\ 2) \langle (1\ 2\ 3) \rangle$
- $(1\ 2) \langle (1\ 2\ 3) \rangle = \{(1\ 2), (2\ 3), (1\ 3)\} = (2\ 3) \langle (1\ 2\ 3) \rangle = (1\ 3) \langle (1\ 2\ 3) \rangle$

Example. In \mathbb{Z} consider the subgroup $4\mathbb{Z} = \{\dots, -4, 0, 4, 8, \dots\}$. This has the following four cosets.

- $0 + 4\mathbb{Z} = \{\dots, -4, 0, 4, 8, \dots\} = 4 + 4\mathbb{Z} = 8 + 4\mathbb{Z} = \dots$
- $1 + 4\mathbb{Z} = \{\dots, -3, 1, 5, 9, \dots\} = 5 + 4\mathbb{Z} = 9 + 4\mathbb{Z} = \dots$
- $2 + 4\mathbb{Z} = \{\dots, -2, 2, 6, 10, \dots\} = 6 + 4\mathbb{Z} = 10 + 4\mathbb{Z} = \dots$
- $3 + 4\mathbb{Z} = \{\dots, -1, 3, 7, 11, \dots\} = 7 + 4\mathbb{Z} = 11 + 4\mathbb{Z} = \dots$

Note. (Nontrivial) **cosets are not subgroups!!!**

Looking at these examples, we can deduce some basic properties of cosets. **Class presentations!**

Proposition. $gH = H$ if and only if $g \in H$.

Proof sketch. H is a subgroup. □

Proposition. $aH = bH$ if and only if $a \in bH$.

Proof sketch. If $a = bh$ then $aH \subset bH$. Also $ah^{-1} = b$, so $b \in aH$ and thus $bH \subset aH$. □

Proposition. $aH = bH$ if and only if $aH \cap bH \neq \emptyset$.

Proof sketch. If $ah_1 = bh_2$ then $a = bh_2h_1^{-1} \in bH$. □

Proposition. $aH = bH$ if and only if $a^{-1}b \in H$.

Proof sketch. If $a^{-1}b = h$ then $b = ah \in aH$. □

Remark. Left cosets are usually not right cosets... But we can say a bit about this relationship.

Proposition. $aH = bH$ if and only if $Ha^{-1} = Hb^{-1}$.

Proof. Consider the following string of equivalent statements.

$$aH = bH$$

$$ah_1 = bh_2$$

$$(ah_1)^{-1} = (bh_2)^{-1}$$

$$h_1^{-1}a^{-1} = h_2^{-1}b^{-1}$$

$$Ha^{-1} = Hb^{-1}$$

□

Corollary. The number of left cosets = number of right cosets.

Using essentially the same argument we can show the following.

Proposition. Numbers of elements also match: $|gH| = |Hg|$.

We'll look again at when left and right cosets are equal when we discuss **normal subgroups**.

Let's get down to business! We want to show that orders of subgroups divide orders of groups. This generalizes the first part of the Fundamental Theorem of Cyclic Groups. I'll present a slick proof which does not rely on your class presentations.

Proposition. Cosets are equivalence classes for an equivalence relation: $a \sim b$ if $a = bh$ for some $h \in H$.

Proof outline. Show reflexive, symmetric, and transitive. □

Corollary. Cosets partition their group G .

Proof. Equivalence classes always partition their set. □

Proposition. All cosets have the same order $|gH| = |H|$.

Proof. The left multiplication map, $\lambda_g : H \rightarrow gH$ has inverse $\lambda_{g^{-1}}$ so it is a bijection. □

Theorem [Lagrange]. The order of a subgroup divides the order of its group.

Proof. G is partitioned by cosets of H , which all have order $|H|$. So $|G| = |H| + \cdots + |H| = m|H|$. □

Definition. The **index** of a subgroup H in a group G is $[G : H] = \frac{|G|}{|H|}$ = "number of cosets of H in G ".

Lagrange's Theorem has a number of immediate implications.

Corollary. For any element of any group, $|g|$ divides $|G|$.

Proof. $|g| = |\langle g \rangle|$ and $\langle g \rangle$ is a subgroup of G . □

Corollary. For any element of any group, $g^n = e$ for $n = |G|$.

Proof. $n = m|g|$, so $g^n = g^{m|g|} = (g^{|g|})^m = (e)^m = e$. □

Corollary (Fermat's Little Theorem). For any integer n and prime p , we have $n^p \equiv n \pmod{p}$

Proof sketch. If n and p are relatively prime, then n generates $\mathbb{Z}_p^{\neq 0}$ multiplicatively. But $|\mathbb{Z}_p^{\neq 0}| = p - 1$. □

Example. We use Fermat's Little Theorem to compute $5^{15} \pmod{7}$ as follows.

$$5^{15} = 5^7 \cdot 5^7 \cdot 5 \equiv 5 \cdot 5 \cdot 5 = 5 \cdot 25 \equiv 5 \cdot 4 = 20 \equiv 6 \pmod{7}$$

Example. We use Fermat's Little Theorem to compute $7^{13} \pmod{11}$ as follows.

$$7^{13} = 7^{11} \cdot 7^2 \equiv 7 \cdot 49 \equiv 7 \cdot 5 = 35 \equiv 2 \pmod{11}$$

Corollary. If G has finite prime order, then G is cyclic!

Proof. If $|G|$ has no divisors, then all elements $g \neq e$ must have order $|G|$. Thus $G = \langle g \rangle$ for any $g \neq e$. □

Corollary. If $K < H < G$ then $[G : K] = [G : H] \cdot [H : K]$.

The third part of the Fundamental Theorem of Cyclic Groups was about **counting** the **number** of subgroups of a given order (only 1 for cyclic groups). This is a bit tricky for general groups, but there is a standard tool for getting an upper bound on the number of subgroups with a given order.

Definition. Given subgroups $H, K < G$ the **product set** is $HK = \{hk \in G \mid h \in H, k \in K\}$.

Note. This is not a group! This is only a set! But we can still use it for counting elements, since $HK \subset G$.

Proposition [Product Formula]. The following relationship holds among orders of sets.

$$|HK| \cdot |H \cap K| = |H| \cdot |K|$$

Proof. Given an $hk \in HK$, every element $x \in H \cap K$ gives a different alternate expression $hk = (hx)(x^{-1}k)$ as a product of $hx \in H$ and $x^{-1}k \in K$. So $|HK| \cdot |H \cap K| \leq |H| \cdot |K|$.

These account for all such rewritings since $h_1k_1 = h_2k_2$ implies $h_2^{-1}h_1 = k_2k_1^{-1} = x \in H \cap K$ such that $h_1k_1 = (h_2x)(x^{-1}k_2)$. So $|HK| \cdot |H \cap K| = |H| \cdot |K|$. □

Corollary. If H and K are subgroups of G then $\frac{|H| \cdot |K|}{|H \cap K|} = |HK| \leq |G|$

We can use this to show **non-existence** of certain subgroups.

Example. A group of order $|G| = np^m$ where p is prime and $n < p$ has at most one subgroup of order p^m .

Proof. If H, K were both subgroups of order p^m then $|H \cap K| \leq p^{m-1}$ ($H \cap K < H$ so order divides p^m). So

$$|G| \geq |HK| = \frac{|H| \cdot |K|}{|H \cap K|} \geq \frac{p^m p^m}{p^{m-1}} = p p^m$$

But $|G| = np^m < p p^m$. □

Example. If $H < G$ where $|H| = 25$ and $|G| = 100$, then any element $g \in G$ with order 5 must be in H .

Proof. If not, then $H \cap \langle g \rangle = \{e\}$. In this case

$$|G| \geq |H \langle g \rangle| = \frac{|H| \cdot |\langle g \rangle|}{|H \cap \langle g \rangle|} = \frac{25 \cdot 5}{1} = 125 > 100$$

□

The second part of the Fundamental Theorem of Cyclic Groups was about **existence**. In cyclic groups, for every divisor of $|G|$ there was a subgroup; however, for general groups this is **NOT TRUE!**

Example. The alternating group A_4 has order $|A_4| = \frac{4!}{2} = 12$... but it has **no** subgroup of order 6.

Proof sketch. First show that any subgroup of index 2 must be **normal**, that is $gH = Hg$ for all $g \in G$ (apply fact that $gH = H$ if and only if $g \in H$). In particular, $gHg^{-1} = H$ for all $g \in G$.

The problem is that there are too many 3-cycles in A_4 ! There are 8 in all: $(1\ 2\ 3)$ and $(1\ 3\ 2)$ fixing 4, and 6 others fixing 1, 2, or 3. If H has order 6, then it contains at least one of these. Applying $gHg^{-1} = H$ then immediately yields five more. But that means $|H| \geq 7$. □

As far as existence of subgroups goes, we can say the following. (We won't prove these theorems until near the end of the semester.)

Theorem [Cauchy]. *There is an element $g \in G$ with order p for every **prime** divisor p of $|G|$.*

Corollary. *In particular, there is a (cyclic) subgroup $\langle g \rangle$ of order p for each **prime** divisor p of $|G|$.*

Theorem [Sylow 1]. *There is a subgroup of order p^k where p^k is the highest power of p dividing $|G|$.*

We could prove Cauchy's Theorem at this point using "orbit / stabilizer" counts, which is very similar to the coset idea we just discussed.

Definition. Given a permutation group $G < S_X$ define the **orbit** of $x \in X$ to be $\text{orbit}_G(x) = \{\sigma(x) \mid \sigma \in G\}$.

Definition. Given $G < S_X$ define the **stabilizer subgroup** of $x \in X$ to be $\text{stab}_G(x) = \{\sigma \in G \mid \sigma(x) = x\}$.

Theorem [Orbit-Stabilizer]. *In this situation $|G| = |\text{orbit}_G(x)| \cdot |\text{stab}_G(x)|$*